more

thys/Untyped_Lambda_Calculus/ILC_Renaming_Equivalence.thy
@@ -19,7 +19,7 @@ inductive reneqv where
 
 thm reneqv_def
 
-(* INSTANTIATING THE Components LOCALE: *)
+(* INSTANTIATING THE CComponents LOCALE: *)
 
 type_synonym T = "itrm \<times> itrm"
 
@@ -29,49 +29,78 @@ definition Tmap :: "(ivar \<Rightarrow> ivar) \<Rightarrow> T \<Rightarrow> T" w
 fun Tfvars :: "T \<Rightarrow> ivar set" where 
 "Tfvars (e1,e2) = FFVars e1 \<union> FFVars e2"
 
+type_synonym B = "ivar dstream option"
 
-interpretation Components where dummy = "undefined :: ivar" and 
-Tmap = Tmap and Tfvars = Tfvars
+fun Bmap :: "(ivar \<Rightarrow> ivar) \<Rightarrow> B \<Rightarrow> B" where 
+"Bmap f xxs = (case xxs of None \<Rightarrow> None
+                          |Some xs \<Rightarrow> Some (dsmap f xs))"
+
+fun Bvars :: "B \<Rightarrow> ivar set" where 
+"Bvars xxs = (case xxs of None \<Rightarrow> {}
+                         |Some xs \<Rightarrow> dsset xs)"
+
+fun wfB :: "B \<Rightarrow> bool" where 
+"wfB xxs = (case xxs of None \<Rightarrow> True
+                       |Some xs \<Rightarrow> super xs)"
+
+definition bsmall :: "ivar set \<Rightarrow> bool" where 
+"bsmall X \<equiv> finite {xs . super xs \<and> X \<inter> dsset xs \<noteq> {}}"
+
+lemma super_dsset_singl: 
+ "super ys \<Longrightarrow> {xs . super xs \<and> dsset ys \<inter> dsset xs \<noteq> {}} = {ys}"
+apply safe 
+apply (meson Int_emptyD super_disj)
+by (simp add: dsset_range)
+
+lemma super_Un_ddset_triv: "{xs. super xs \<and> (A \<union> B) \<inter> dsset xs \<noteq> {}} \<subseteq>  
+   {xs. super xs \<and> A \<inter> dsset xs \<noteq> {}} \<union> 
+   {xs. super xs \<and> B \<inter> dsset xs \<noteq> {}}"
+by auto
+
+interpretation CComponents where dummy = "undefined :: ivar" and 
+Tmap = Tmap and Tfvars = Tfvars and Bmap = Bmap and Bvars = Bvars 
+and wfB = wfB and bsmall = bsmall
 apply standard unfolding ssbij_def Tmap_def  
-  using small_Un small_def iterm.card_of_FFVars_bounds
-  apply (auto simp: iterm.rrename_id0s map_prod.comp iterm.rrename_comp0s inf_A)
-  using var_sum_class.Un_bound by blast
+using small_Un small_def iterm.card_of_FFVars_bounds
+apply (auto simp: iterm.rrename_id0s map_prod.comp 
+iterm.rrename_comp0s inf_A bsmall_def intro!: ext split: option.splits)
+apply (simp add: iterm.set_bd_UNIV) 
+apply (simp add: comp_def dstream.map_comp)
+apply (simp add: dstream_map_ident_strong)
+unfolding bsmall_def apply(frule super_dsset_singl) apply auto
+using super_Un_ddset_triv  
+by (smt (verit) finite_Un rev_finite_subset) 
 
-definition G :: "(T \<Rightarrow> bool) \<Rightarrow> ivar set \<Rightarrow> T \<Rightarrow> bool"
+definition G :: "(T \<Rightarrow> bool) \<Rightarrow> B \<Rightarrow> T \<Rightarrow> bool"
 where
-"G \<equiv> \<lambda>R B t.  
-         (\<exists>xs x x'. B = {} \<and> fst t = iVar x \<and> snd t = iVar x' \<and> 
+"G \<equiv> \<lambda>R xxs t.  
+         (\<exists>xs x x'. xxs = None \<and> fst t = iVar x \<and> snd t = iVar x' \<and> 
                     super xs \<and> {x,x'} \<subseteq> dsset xs) 
          \<or>
-         (\<exists>xs e e'. B = dsset xs \<and> fst t = iLam xs e \<and> snd t = iLam xs e' \<and> 
+         (\<exists>xs e e'. xxs = Some xs \<and> fst t = iLam xs e \<and> snd t = iLam xs e' \<and> 
                     super xs \<and> R (e,e'))
          \<or> 
-         (\<exists>e1 e1' es2 es2'. B = {} \<and> fst t = iApp e1 es2 \<and> snd t = iApp e1' es2' \<and> 
+         (\<exists>e1 e1' es2 es2'. xxs = None \<and> fst t = iApp e1 es2 \<and> snd t = iApp e1' es2' \<and> 
                             R (e1,e1') \<and> (\<forall>e e'. {e,e'} \<subseteq> sset es2 \<union> sset es2' \<longrightarrow> R (e,e')))"
  
 
 (* VERIFYING THE HYPOTHESES FOR BARENDREGT-ENHANCED INDUCTION: *)
 
-lemma G_mmono: "R \<le> R' \<Longrightarrow> small B \<Longrightarrow> G R B t \<Longrightarrow> G R' B t"
+lemma G_mmono: "R \<le> R' \<Longrightarrow> G R xxs t \<Longrightarrow> G R' xxs t"
 unfolding G_def by fastforce
 
 
-definition wfBij where "wfBij \<sigma> \<equiv> \<forall>xs. super xs \<longleftrightarrow> super (dsmap \<sigma> xs)"
-(* we defined closedness looking at the possible values of B in G: *)
-definition closed where "closed X \<equiv> X = {} \<or> (\<exists>xs. super xs \<and> X = dsset xs)"
-(* no need for this more elaborate setting: *)
-(* \<forall>xs. super xs \<and> dsset xs \<inter> X \<noteq> {} \<longrightarrow> dsset xs \<subseteq> X *)
-
-
 (* NB: Everything is passed \<sigma>-renamed as witnesses to exI *)
-lemma G_eequiv: "ssbij \<sigma> \<Longrightarrow> wfBij \<sigma> \<Longrightarrow> small B \<Longrightarrow> G R B t \<Longrightarrow> G (\<lambda>t'. R (Tmap (inv \<sigma>) t')) (image \<sigma> B) (Tmap \<sigma> t)"
+lemma G_eequiv: 
+"ssbij \<sigma> \<Longrightarrow> wfBij \<sigma> \<Longrightarrow> G R xxs t \<Longrightarrow> 
+ G (\<lambda>t'. R (Tmap (inv \<sigma>) t')) (Bmap \<sigma> xxs) (Tmap \<sigma> t)"
 unfolding G_def apply(elim disjE)
   subgoal apply(rule disjI3_1)
   subgoal apply(elim exE) subgoal for xs x x'
   apply(rule exI[of _ "dsmap \<sigma> xs"]) 
   apply(rule exI[of _ "\<sigma> x"]) apply(rule exI[of _ "\<sigma> x'"]) 
   apply(cases t) unfolding ssbij_def small_def Tmap_def wfBij_def
-  by simp . .
+  apply simp by (metis option.simps(5)) . .
   (* *)
   subgoal apply(rule disjI3_2)
   subgoal apply(elim exE) subgoal for xs e e'
@@ -79,7 +108,7 @@ unfolding G_def apply(elim disjE)
   apply(rule exI[of _ "rrename \<sigma> e"]) 
   apply(rule exI[of _ "rrename \<sigma> e'"])  
   apply(cases t) unfolding ssbij_def small_def Tmap_def wfBij_def
-  by (simp add: iterm.rrename_comps) . . 
+  apply (simp add: iterm.rrename_comps) by (metis option.simps(5)) . . 
   (* *)
   subgoal apply(rule disjI3_3)
   subgoal apply(elim exE) subgoal for e1 e1' es2 es2'
@@ -89,100 +118,135 @@ unfolding G_def apply(elim disjE)
   apply (simp add: iterm.rrename_comps) 
   by (metis image_in_bij_eq iterm.rrename_bijs iterm.rrename_inv_simps) . . .
 
-lemma Tvars_dsset: "(Tfvars t - dsset xs) \<inter> dsset xs = {}" "|Tfvars t - dsset xs| <o |UNIV::ivar set|"
-apply auto by (meson card_of_minus_bound small_Tfvars small_def)
+
 
 (* *)
 
-lemma G_closed: "G R B t \<Longrightarrow> closed B"
-unfolding G_def closed_def by auto 
+lemma G_wfB: "G R B t \<Longrightarrow> wfB B"
+unfolding G_def by auto 
 
-lemma wfBij_id[simp,intro]: "wfBij id" unfolding wfBij_def by simp
 
-lemma wfBij_comp[simp]: "ssbij \<sigma> \<Longrightarrow> wfBij \<sigma> \<Longrightarrow> ssbij \<tau> \<Longrightarrow> wfBij \<tau> \<Longrightarrow> wfBij (\<tau> o \<sigma>)"
-unfolding wfBij_def by (metis ssbij_def dstream.map_comp)
+lemma extend_super: 
+assumes "super xs" "|A| <o |UNIV::ivar set|" 
+ "finite {xs. super xs \<and> A \<inter> dsset xs \<noteq> {}}" "A' \<subseteq> A" "dsset xs \<inter> A' = {}"
+shows "\<exists>\<rho>. bij (\<rho>::ivar\<Rightarrow>ivar) \<and> |supp \<rho>| <o |UNIV::ivar set| \<and> (\<forall>xs. super xs \<longleftrightarrow> super (dsmap \<rho> xs)) \<and> \<rho> ` (dsset xs) \<inter> A = {} \<and> id_on A' \<rho>"
+sorry
 
-lemma wfBij_inv[simp]: "ssbij \<sigma> \<Longrightarrow> wfBij \<sigma> \<Longrightarrow> wfBij (inv \<sigma>)"
-unfolding wfBij_def ssbij_def 
-by (metis bij_imp_bij_inv dstream.map_comp dstream.map_id inv_inv_eq inv_o_simp1 supp_inv_bound)
-
-lemma dsset_dsmap_inv_NE: "bij \<sigma> \<Longrightarrow> dsset xs \<inter> \<sigma> ` A \<noteq> {} \<longleftrightarrow> dsset (dsmap (inv \<sigma>) xs) \<inter> A \<noteq> {}"
-by (metis bij_betw_def bij_imp_bij_betw bij_imp_bij_inv dsset_dsmap image_Int_empty inf_commute)
-
-lemma closed_wfBij: "ssbij \<sigma> \<Longrightarrow> wfBij \<sigma> \<Longrightarrow> closed A \<Longrightarrow> closed (\<sigma> ` A)"
-unfolding closed_def apply clarify  
-by (metis ILC2.ssbij_def dstream.set_map wfBij_def)
-(*
-  subgoal for xs x  apply(subst image_in_bij_eq)
-    subgoal unfolding ssbij_def by simp
-    subgoal apply(frule wfBij_inv)
-      subgoal by simp
-      subgoal apply(subst (asm) dsset_dsmap_inv_NE)
-        subgoal unfolding ssbij_def by simp
-        subgoal by (metis ILC2.ssbij_def IntD2 bij_bij_betw_inv dstream.set_map inf.absorb1 
-                    rev_image_eqI supp_inv_bound wfBij_def) . . . . 
-*)
-
-(* *)
-lemma small_ssbij_closed: 
-assumes s: "small A" "small B" "small A'" "A \<inter> A' = {}" and c: "closed A" 
-shows "\<exists>\<rho>. ssbij \<rho> \<and> wfBij \<rho> \<and> \<rho> ` A \<inter> B = {} \<and> (\<forall>a\<in>A'. \<rho> a = a)" 
-using c unfolding closed_def proof(elim disjE exE conjE)
-  assume A: "A = {}"
-  show ?thesis apply(rule exI[of _ id]) unfolding A ssbij_def by auto
+lemma eextend_to_wfBij: 
+assumes "wfB xxs" "small A" "bsmall A" "A' \<subseteq> A" "Bvars xxs \<inter> A' = {}"
+shows "\<exists>\<rho>. ssbij \<rho> \<and> wfBij \<rho> \<and> \<rho> ` Bvars xxs \<inter> A = {} \<and> id_on A' \<rho>" 
+proof(cases xxs)
+  case None
+  thus ?thesis apply(intro exI[of _ id]) unfolding ssbij_def by auto
 next
-  fix xs assume xs: "super xs" and A: "A = dsset xs"
-  obtain xs' where xs': "super xs'" and xss': "xs \<noteq> xs'" and "dsset xs' \<inter> B = {}"
-  using xs super_infinite sledgehammer
- by (ssmt (verit, del_insts) Collect_cong Collect_conv_if finite.simps)
-  hence ds: "dsset xs \<inter> dsset xs' = {}" using super_disj xs by auto
-  show ?thesis
-  sorry
-qed
+  case (Some xs)
+  hence 0: "super xs" "|A| <o |UNIV::ivar set|" "finite {xs. super xs \<and> A \<inter> dsset xs \<noteq> {}}" "A' \<subseteq> A"
+  "dsset xs \<inter> A' = {}"
+  using assms by (auto split: option.splits simp: small_def bsmall_def) 
+  show ?thesis using extend_super[OF 0] apply safe
+  subgoal for \<rho> apply(rule exI[of _ \<rho>]) 
+  using Some by (auto split: option.splits simp: wfBij_def ssbij_def) .
+qed 
+
+
+interpretation Reneqv : IInduct1 
+where dummy = "undefined :: ivar" and 
+Tmap = Tmap and Tfvars = Tfvars and Bmap = Bmap and Bvars = Bvars 
+and wfB = wfB and bsmall = bsmall and GG = G
+apply standard
+using G_mmono G_eequiv G_wfB eextend_to_wfBij by auto
+
+
+(* *)
+
+lemma reneqv_I: "reneqv t1 t2 = Reneqv.II (t1,t2)" 
+unfolding reneqv_def Reneqv.II_def lfp_curry2 apply(rule arg_cong2[of _ _ _ _ lfp], simp_all)
+unfolding fun_eq_iff G_def apply clarify
+subgoal for R tt1 tt2 apply(rule iffI)
+  subgoal apply(elim disjE exE conjE)
+    \<^cancel>\<open>iVar: \<close>
+    subgoal for xs x x' apply(rule exI[of _ None]) apply(rule disjI3_1) by auto
+    \<^cancel>\<open>iLam: \<close> 
+    subgoal for xs e e' apply(rule exI[of _ "Some xs"]) apply(rule disjI3_2) by auto 
+    \<^cancel>\<open>iApp: \<close>
+    subgoal apply(rule exI[of _ None]) apply(rule disjI3_3) by auto .
+    (* *)
+  subgoal apply(elim disjE exE conjE)
+    \<^cancel>\<open>iVar: \<close>
+    subgoal apply(rule disjI3_1) by auto
+    \<^cancel>\<open>iLam: \<close>
+    subgoal apply(rule disjI3_2) by auto
+    \<^cancel>\<open>iApp: \<close>
+    subgoal apply(rule disjI3_3) by auto . . .
   
+lemma reneqv_FFvars_super: 
+"reneqv e1 e2 \<Longrightarrow> 
+  {xs. super xs \<and> FFVars e1 \<inter> dsset xs \<noteq> {}} = {xs. super xs \<and> FFVars e2 \<inter> dsset xs \<noteq> {}} 
+  \<and>
+  finite {xs. super xs \<and> FFVars e1 \<inter> dsset xs \<noteq> {}} \<and> 
+  finite {xs. super xs \<and> FFVars e2 \<inter> dsset xs \<noteq> {}}"
+sorry
+
+lemma III_bsmall: "Reneqv.II t \<Longrightarrow> bsmall (Tfvars t)"
+apply(cases t)
+  subgoal for e1 e2 apply simp
+  unfolding reneqv_I[symmetric] apply(drule reneqv_FFvars_super)
+  unfolding bsmall_def[symmetric] 
+  using bsmall_Un by auto .
+
 
 
 thm refresh
 lemma refresh_super: 
-assumes V: "V \<inter> dsset xs = {}" "|V| <o |UNIV::ivar set|" "super xs"  
-shows "\<exists>f xs'. bij (f::ivar\<Rightarrow>ivar) \<and> |supp f| <o |UNIV::ivar set| \<and> 
-               dsset xs' \<inter> dsset xs = {} \<and> dsset xs' \<inter> V = {} \<and>
-               dsmap f xs = xs' \<and> id_on V f \<and> (\<forall>ys. super ys \<longleftrightarrow> super (dsmap f ys))"
-proof-
-  define A A' B where A: "A \<equiv> dsset xs" and A': "A' = V" and B: "B \<equiv> V \<union> dsset xs"
-  have 0: "small A" "small B" "small A'" "A \<inter> A' = {}" "closed A"
-  unfolding A A' B closed_def using V 
-  apply auto 
-  using small_Un small_def apply blast
-  using small_def super_disj by fastforce+
-  show ?thesis using small_ssbij_closed[OF 0] 
-  apply safe subgoal for f apply(intro exI[of _ f] exI[of _ "dsmap f xs"]) 
-  unfolding ssbij_def wfBij_def A A' B id_on_def by auto .
-qed
+assumes V: " dsset xs \<inter> V = {}" "|V| <o |UNIV::ivar set|" 
+  "finite {xs. super xs \<and> V \<inter> dsset xs \<noteq> {}}"
+and xs: "super xs"  
+shows "\<exists>f. bij (f::ivar\<Rightarrow>ivar) \<and> |supp f| <o |UNIV::ivar set| \<and> 
+               \<comment> \<open> dsset xs' \<inter> dsset xs = {} \<and>  \<close>dsset (dsmap f xs) \<inter> V = {} \<and>
+           id_on V f \<and> (\<forall>ys. super ys \<longleftrightarrow> super (dsmap f ys))"
+using extend_super[OF xs V(2) V(3) _ V(1), simplified]
+apply safe subgoal for \<rho> apply(intro exI[of _ \<rho>]) 
+unfolding id_on_def by auto .
+
+
+lemma Tvars_dsset: "dsset xs \<inter> (Tfvars t - dsset xs) = {}" 
+  "|Tfvars t - dsset xs| <o |UNIV::ivar set|"
+using ILC2.small_def card_of_minus_bound ssmall_Tfvars by blast+
+
+lemma Tvars_dsset_finite: "Reneqv.II t \<Longrightarrow> finite {xs. super xs \<and> (Tfvars t - dsset ys) \<inter> dsset (xs::ivar dstream) \<noteq> {}}"
+apply(subgoal_tac "bsmall (Tfvars t)")
+  subgoal unfolding bsmall_def 
+    by (smt (verit) Collect_mono Diff_Int_distrib2 empty_Diff rev_finite_subset)
+  subgoal by (metis III_bsmall) . 
 
 lemma G_rrefresh: 
-"(\<forall>\<sigma> t. ssbij \<sigma> \<and> wfBij \<sigma> \<and> R t \<longrightarrow> R (Tmap \<sigma> t)) \<Longrightarrow> small B \<Longrightarrow> G R B t \<Longrightarrow> 
- \<exists>C. small C \<and> C \<inter> Tfvars t = {} \<and> G R C t"
-apply(frule G_closed)
+"(\<forall>t. R t \<longrightarrow> Reneqv.II t) \<Longrightarrow> 
+ (\<forall>\<sigma> t. ssbij \<sigma> \<and> wfBij \<sigma> \<and> R t \<longrightarrow> R (Tmap \<sigma> t)) \<Longrightarrow> 
+ G R xxs t \<Longrightarrow> 
+ \<exists>yys. Bvars yys \<inter> Tfvars t = {} \<and> G R yys t"
+apply(subgoal_tac "Reneqv.II t") defer
+apply (metis Reneqv.GG_mmono2 Reneqv.II.simps predicate1I)
+subgoal premises p using p apply-
+apply(frule G_wfB)
 unfolding G_def Tmap_def apply safe
-  subgoal for xs x x'
-  apply(rule exI[of _ "{}"])  
+  subgoal for xs x x' 
+  apply(rule exI[of _ None])  
   apply(intro conjI)
-    subgoal by simp
-    subgoal unfolding ssbij_def small_def by auto 
+    subgoal by simp 
     subgoal apply(rule disjI3_1) 
     apply(rule exI[of _ xs]) 
     apply(rule exI[of _ x])
     apply(rule exI[of _ x']) 
     apply(cases t) apply simp . .
   (* *)
-  subgoal for xs e e'
-  apply(frule refresh_super[OF Tvars_dsset, of xs t]) apply safe
+  subgoal for xs e e' 
+  apply(frule refresh_super[OF Tvars_dsset Tvars_dsset_finite[OF p(4)]])
+  apply safe
   subgoal for f
-  apply(rule exI[of _ "f ` (dsset xs)"])  
-  apply(intro conjI)
-    subgoal using small_dsset small_image by auto
-    subgoal unfolding id_on_def by auto (metis DiffI Int_emptyD image_eqI)
+  apply(rule exI[of _ "Some (dsmap f xs)"])  
+  apply(intro conjI) 
+    subgoal unfolding id_on_def apply auto  
+      by (smt (verit, ccfv_SIG) Diff_Int_distrib Diff_disjoint Diff_empty Int_emptyD Tfvars.simps Un_iff bij_betw_apply bij_imp_bij_betw dstream.set_map iterm.set(3) prod.collapse super_disj)
     subgoal apply(rule disjI3_2)
     apply(rule exI[of _ "dsmap f xs"]) 
     apply(rule exI[of _ "rrename f e"]) 
@@ -194,57 +258,38 @@ unfolding G_def Tmap_def apply safe
         subgoal unfolding ssbij_def by auto
         subgoal by (smt (verit, best) Diff_iff Un_iff iLam_rrename id_on_def 
            rrename_eq_itvsubst_iVar) . 
-        subgoal unfolding id_on_def ssbij_def wfBij_def by auto . . .
+        subgoal unfolding id_on_def ssbij_def wfBij_def by (auto split: option.splits) . . .
   (* *)
   subgoal for e1 e1' es2 es2'
-  apply(rule exI[of _ "{}"])  
+  apply(rule exI[of _ None])  
   apply(intro conjI)
-    subgoal by simp
-    subgoal unfolding ssbij_def small_def by auto 
+    subgoal by simp 
     subgoal apply(rule disjI3_3) 
     apply(rule exI[of _ "e1"]) 
     apply(rule exI[of _ "e1'"])
     apply(rule exI[of _ "es2"]) 
     apply(rule exI[of _ "es2'"]) 
-    apply(cases t) by simp . . 
+    apply(cases t) by simp . . .
  
 
 (* FINALLY, INTERPRETING THE IInduct LOCALE: *)
 
-interpretation Reneqv : IInduct where dummy = "undefined :: ivar" and 
-Tmap = Tmap and Tfvars = Tfvars and G = G and closed = closed and wfBij = wfBij 
-apply standard 
-  using G_mmono G_eequiv 
-  G_closed wfBij_id wfBij_comp wfBij_inv closed_wfBij small_ssbij_closed
-  G_rrefresh by auto  
+interpretation Reneqv : IInduct
+where dummy = "undefined :: ivar" and 
+Tmap = Tmap and Tfvars = Tfvars and Bmap = Bmap and Bvars = Bvars 
+and wfB = wfB and bsmall = bsmall and GG = G
+apply standard using III_bsmall G_rrefresh by auto
 
 (* *)
 
-lemma reneqv_I: "reneqv t1 t2 = Reneqv.I (t1,t2)" 
-unfolding reneqv_def Reneqv.I_def lfp_curry2 apply(rule arg_cong2[of _ _ _ _ lfp], simp_all)
-unfolding fun_eq_iff G_def apply clarify
-subgoal for R tt1 tt2 apply(rule iffI)
-  subgoal apply(elim disjE exE conjE)
-    \<^cancel>\<open>iVar: \<close>
-    subgoal for xs x x' apply(rule exI[of _ "{}"], rule conjI, simp) apply(rule disjI3_1) by auto
-    \<^cancel>\<open>iLam: \<close> 
-    subgoal for xs e e' apply(rule exI[of _ "dsset xs"], rule conjI, simp) apply(rule disjI3_2) by auto 
-    \<^cancel>\<open>iApp: \<close>
-    subgoal apply(rule exI[of _ "{}"], rule conjI, simp) apply(rule disjI3_3) by auto .
-    (* *)
-  subgoal apply(elim disjE exE conjE)
-    \<^cancel>\<open>iVar: \<close>
-    subgoal apply(rule disjI3_1) by auto
-    \<^cancel>\<open>iLam: \<close>
-    subgoal apply(rule disjI3_2) by auto
-    \<^cancel>\<open>iApp: \<close>
-    subgoal apply(rule disjI3_3) by auto . . .
 
 (* FROM ABSTRACT BACK TO CONCRETE: *)
 thm reneqv.induct[no_vars] 
 
+thm bsmall_def[of "Pfvars p"]
+
 corollary BE_induct_reneqv: 
-assumes par: "\<And>p. small (Pfvars p)"
+assumes par: "\<And>p. small (Pfvars p) \<and> finite {xs. super xs \<and> Pfvars p \<inter> dsset xs \<noteq> {}}"
 and st: "reneqv t1 t2"  
 and iVar: "\<And>xs x x' p. 
   super xs \<Longrightarrow> {x,x'} \<subseteq> dsset xs \<Longrightarrow>
@@ -261,7 +306,8 @@ shows "R p t1 t2"
 unfolding reneqv_I
 apply(subgoal_tac "case (t1,t2) of (t1, t2) \<Rightarrow> R p t1 t2")
   subgoal by simp
-  subgoal using par st apply(elim Reneqv.BE_induct[where R = "\<lambda>p (t1,t2). R p t1 t2"])
+  subgoal using par st 
+  unfolding bsmall_def[symmetric] apply(elim Reneqv.BE_iinduct[where R = "\<lambda>p (t1,t2). R p t1 t2"])
     subgoal unfolding reneqv_I by simp
     subgoal for p B t apply(subst (asm) G_def) 
     unfolding reneqv_I[symmetric] apply(elim disjE exE)
